WIP defining mupd modality

src/MonotonePCM.v
@@ -711,6 +711,458 @@ Section MAP.
 End MAP.
 
 
+From iris.bi Require Import derived_laws. Import bi.
+
+Section MUPD.
+  Definition mset := list nat.
+  Definition mset_disjoint (s0 s1: mset): Prop :=
+    forall n (IN0: List.In n s0) (IN1: List.In n s1), False.
+
+  Fixpoint mset_disjoint_b (s0 s1: mset): bool :=
+    match s0 with
+    | [] => true
+    | hd::tl =>
+        match find (Nat.eqb hd) s1 with
+        | Some _ => false
+        | None => mset_disjoint_b tl s1
+        end
+    end.
+
+  Lemma mset_disjoint_b_reflect s0 s1
+    :
+    mset_disjoint s0 s1 <-> mset_disjoint_b s0 s1 = true.
+  Proof.
+    induction s0; ss.
+    { split; i; auto. ii. inv IN0. }
+    des_ifs.
+    { split; i.
+      { eapply find_some in Heq. des.
+        rewrite Nat.eqb_eq in Heq0. subst.
+        exfalso. eapply H; eauto. econs; ss.
+      }
+      { ii. inv IN0; eauto. }
+    }
+    { rewrite <- IHs0. split; i.
+      { ii. eapply H; eauto. econs 2; ss. }
+      { ii. inv IN0.
+        { eapply find_none in Heq; eauto. rewrite Nat.eqb_refl in Heq. ss. }
+        { eapply H; eauto. }
+      }
+    }
+  Qed.
+
+  Definition mset_sub (s0 s1: mset): Prop :=
+    exists s, Permutation (s ++ s0) s1.
+
+  Global Program Instance mset_sub_PreOrder: PreOrder mset_sub.
+  Next Obligation.
+  Proof.
+    ii. exists []. ss.
+  Qed.
+  Next Obligation.
+  Proof.
+    ii. unfold mset_sub in *. des.
+    rewrite <- H in H0. exists (s ++ s0).
+    rewrite <- app_assoc. auto.
+  Qed.
+
+  Definition mset_minus (s0 s1: mset): mset :=
+    match list_remove_list s0 s1 with
+    | Some s => s
+    | None => []
+    end.
+
+  Definition mset_sub_b (s0 s1: mset): bool :=
+    match list_remove_list s0 s1 with
+    | Some _ => true
+    | None => false
+    end.
+
+  Lemma list_remove_none A `{EqDecision A} (a: A) (l: list A)
+        (NONE: list_remove a l = None)
+    :
+    ~ List.In a l.
+  Proof.
+    revert NONE. induction l; ss.
+    des_ifs. i. unfold fmap, option_fmap, option_map in NONE.
+    des_ifs. ii. des; clarify. eapply IHl; auto.
+  Qed.
+
+  Lemma mset_sub_b_reflect s0 s1
+    :
+    mset_sub s0 s1 <-> mset_sub_b s0 s1 = true.
+  Proof.
+    revert s1. induction s0; ss; i.
+    { split; i; auto. exists s1. rewrite app_nil_r. auto. }
+    { unfold mset_sub_b in *. ss.
+      destruct (list_remove a s1) eqn:EQ; ss.
+      { eapply list_remove_Some in EQ.
+        rewrite <- IHs0. unfold mset_sub. split.
+        { i. des. rewrite EQ in H.
+          rewrite <- Permutation_middle in H.
+          apply Permutation_cons_inv in H.
+          exists s. auto.
+        }
+        { i. des. rewrite <- H in EQ.
+          eexists s. rewrite EQ. rewrite <- Permutation_middle. auto.
+        }
+      }
+      { eapply list_remove_none in EQ. split; i; ss.
+        exfalso. unfold mset_sub in H. des.
+        rewrite <- Permutation_middle in H.
+        eapply EQ. eapply Permutation_in; eauto.
+        econs; ss.
+      }
+    }
+  Qed.
+
+  Context `{Σ: GRA.t}.
+  Variable I: nat -> iProp.
+  Definition mset_all (l: mset) := fold_right (fun n P => I n ** P) True%I l.
+
+  Lemma mset_all_nil
+    :
+    ⊢ mset_all [].
+  Proof.
+    unfold mset_all. ss. auto.
+  Qed.
+
+  Lemma mset_all_cons_fold hd tl
+    :
+    (I hd ** mset_all tl)
+      -∗
+      (mset_all (hd::tl)).
+  Proof.
+    unfold mset_all. ss.
+  Qed.
+
+  Lemma mset_all_cons_unfold hd tl
+    :
+    (mset_all (hd::tl))
+      -∗
+      (I hd ** mset_all tl).
+  Proof.
+    unfold mset_all. ss.
+  Qed.
+
+  Lemma mset_all_split l0 l1
+    :
+    (mset_all (l0 ++ l1))
+      -∗
+      (mset_all l0 ** mset_all l1).
+  Proof.
+    induction l0; ss.
+    { iIntros "SAT". iFrame. }
+    { iIntros "[INTERP SAT]". iFrame. iApply IHl0; auto. }
+  Qed.
+
+  Lemma mset_all_combine l0 l1
+    :
+    (mset_all l0 ** mset_all l1)
+      -∗
+      (mset_all (l0 ++ l1)).
+  Proof.
+    induction l0; ss.
+    { iIntros "[_ SAT]". auto. }
+    { iIntros "[[INTERP SAT0] SAT1]". iFrame.
+      iApply IHl0. iFrame.
+    }
+  Qed.
+
+  Lemma mset_all_add l a
+    :
+    (I a ** mset_all l)
+      -∗
+      (mset_all (l++[a])).
+  Proof.
+    iIntros "[NEW SAT]". iApply mset_all_combine. iFrame.
+  Qed.
+
+  Lemma mset_all_permutation l0 l1
+        (PERM: Permutation l0 l1)
+    :
+    mset_all l0 ⊢ mset_all l1.
+  Proof.
+    induction PERM.
+    { auto. }
+    { iIntros "H". iApply mset_all_cons_fold.
+      iPoseProof (mset_all_cons_unfold with "H") as "[HD TL]".
+      iFrame. iApply IHPERM; auto.
+    }
+    { iIntros "H". iApply mset_all_cons_fold.
+      iPoseProof (mset_all_cons_unfold with "H") as "[HD0 TL]".
+      iPoseProof (mset_all_cons_unfold with "TL") as "[HD1 TL]".
+      iSplitL "HD1"; auto. iApply mset_all_cons_fold. iFrame.
+    }
+    { etrans; eauto. }
+  Qed.
+
+  Lemma mset_all_sub l0 l1
+        (SUB: mset_sub l0 l1)
+    :
+    mset_all l1 ⊢ mset_all l0 ** (mset_all l0 -* mset_all l1).
+  Proof.
+    red in SUB. des. iIntros "H".
+    iPoseProof (mset_all_permutation with "H") as "H".
+    { symmetry. eauto. }
+    iPoseProof (mset_all_split with "H") as "[H0 H1]". iFrame.
+    iIntros "H1". iApply mset_all_permutation; eauto.
+    iApply mset_all_combine. iFrame.
+  Qed.
+
+  Lemma mset_all_update l k a
+        (FIND: nth_error l k = Some a)
+    :
+    mset_all l ⊢ I a ** (I a -* mset_all l).
+  Proof.
+    hexploit nth_error_split; eauto. i. des. subst.
+    iIntros "SAT". iPoseProof (mset_all_split with "SAT") as "[SAT0 SAT1]".
+    iPoseProof (mset_all_cons_unfold with "SAT1") as "[OLD SAT1]".
+    iFrame. iIntros "NEW". iApply mset_all_combine. iFrame.
+  Qed.
+
+  Lemma mset_all_nth_sub l k a
+        (FIND: nth_error l k = Some a)
+    :
+    ⊢ SubIProp (I a) (mset_all l).
+  Proof.
+    iIntros "H". iPoseProof (mset_all_update with "H") as "[H0 H1]"; eauto.
+    iFrame. iModIntro. iIntros "H". iModIntro. iApply ("H1" with "H").
+  Qed.
+
+  Definition MUpd (l0 l1: mset) (P: iProp): iProp :=
+    mset_all l0 -* #=> (mset_all l1 ** P).
+
+  Lemma MUpd_mask_subseteq E1 E2 :
+    mset_sub E2 E1 -> ⊢ MUpd E1 E2 (MUpd E2 E1 emp).
+  Proof.
+    i. iIntros "H".
+    iPoseProof (mset_all_sub with "H") as "[H0 H1]"; eauto.
+    iModIntro. iFrame. iIntros "H0". iModIntro. iSplit; auto.
+    iApply "H1"; auto.
+  Qed.
+
+  Lemma MUpd_mono E1 E2 P Q
+    :
+    (P ⊢ Q) -> (MUpd E1 E2 P ⊢ MUpd E1 E2 Q).
+  Proof.
+    i. iIntros "H0 H1". iPoseProof ("H0" with "H1") as "> [H0 H1]".
+    iModIntro. iFrame. iApply H. auto.
+  Qed.
+
+  Lemma MUpd_trans E1 E2 E3 P
+    :
+    MUpd E1 E2 (MUpd E2 E3 P) ⊢ MUpd E1 E3 P.
+  Proof.
+    iIntros "H0 H1". iPoseProof ("H0" with "H1") as "> [H0 H1]".
+    iPoseProof ("H1" with "H0") as "> [H0 H1]".
+    iModIntro. iFrame.
+  Qed.
+
+  Lemma MUpd_frame_r E1 E2 P R
+    :
+    MUpd E1 E2 P ** R ⊢ MUpd E1 E2 (P ** R).
+  Proof.
+    iIntros "[H0 H1] H2". iPoseProof ("H0" with "H2") as "> [H0 H2]".
+    iModIntro. iFrame.
+  Qed.
+
+  Lemma MUpd_mask_frame_r' E1 E2 Ef P
+    :
+    (MUpd E1 E2 P ⊢ MUpd (E1 ++ Ef) (E2 ++ Ef) P).
+  Proof.
+    i. iIntros "H0 H1".
+    iPoseProof (mset_all_split with "H1") as "[H1 H2]".
+    iPoseProof ("H0" with "H1") as "> [H0 H1]".
+    iModIntro. iFrame. iApply (mset_all_combine with "[H2 H0]"). iFrame.
+  Qed.
+
+  Global Instance MUpd_ne E1 E2 : NonExpansive (MUpd E1 E2).
+  Proof.
+    ii. unfold MUpd. rewrite H. auto.
+  Qed.
+
+  Global Instance MUpd_proper E1 E2 :
+    Proper ((≡) ==> (≡)) (MUpd E1 E2) := ne_proper _.
+
+  Global Instance MUpd_mono' E1 E2 : Proper ((⊢) ==> (⊢)) (MUpd E1 E2).
+  Proof. intros P Q; apply MUpd_mono. Qed.
+  Global Instance MUpd_flip_mono' E1 E2 :
+    Proper (flip (⊢) ==> flip (⊢)) (MUpd E1 E2).
+  Proof. intros P Q; apply MUpd_mono. Qed.
+
+  Lemma MUpd_mask_intro_subseteq E1 E2 P :
+    mset_sub E2 E1 -> P ⊢ MUpd E1 E2 (MUpd E2 E1 P).
+  Proof.
+    intros HE. iIntros "H0". iApply MUpd_mono.
+    { eapply MUpd_mono. instantiate (1:=emp ** P).
+      iIntros "[H0 H1]". auto.
+    }
+    { iApply MUpd_mono.
+      { iApply MUpd_frame_r. }
+      iApply MUpd_frame_r. iFrame.
+      iApply MUpd_mask_subseteq. auto.
+    }
+  Qed.
+
+  Lemma MUpd_intro E P : P ⊢ MUpd E E P.
+  Proof.
+    etrans.
+    { eapply MUpd_mask_intro_subseteq. reflexivity. }
+    { eapply MUpd_trans. }
+  Qed.
+
+  Lemma MUpd_idemp E P : (MUpd E E (MUpd E E P)) ⊣⊢ MUpd E E P.
+  Proof.
+    apply: anti_symm.
+    - apply MUpd_trans.
+    - apply MUpd_intro.
+  Qed.
+
+  Lemma MUpd_mask_weaken {E1} E2 {E3 P} :
+    mset_sub E2 E1 ->
+    (MUpd E2 E1 emp -* MUpd E2 E3 P) -∗ MUpd E1 E3 P.
+  Proof.
+    intros HE.
+    iIntros "H1".
+    iPoseProof MUpd_mask_subseteq as "H0"; eauto.
+    iPoseProof (MUpd_frame_r with "[H0 H1]") as "H".
+    { iSplitR "H1".
+      { iExact "H0". }
+      { iExact "H1". }
+    }
+    iApply MUpd_trans. iClear "H0".
+    iStopProof. eapply MUpd_mono.
+    eapply wand_elim_r.
+  Qed.
+
+  Lemma MUpd_mask_intro E1 E2 P :
+    mset_sub E2 E1 ->
+    ((MUpd E2 E1 emp) -∗ P) -∗ MUpd E1 E2 P.
+  Proof.
+    intros. etrans; [|by apply MUpd_mask_weaken].
+    rewrite <- MUpd_intro. auto.
+  Qed.
+
+  Lemma MUpd_mask_intro_discard E1 E2 P:
+    mset_sub E2 E1 -> P ⊢ MUpd E1 E2 P.
+  Proof.
+    intros. etrans; [|by apply MUpd_mask_intro].
+    apply Wand_intro_r. rewrite sep_elim_l; try done.
+    econs 2. typeclasses eauto.
+  Qed.
+
+  Lemma MUpd_frame_l E1 E2 R Q : (R ∗ MUpd E1 E2 Q) ⊢ MUpd E1 E2 (R ∗ Q).
+  Proof. rewrite !(comm _ R); apply MUpd_frame_r. Qed.
+  Lemma MUpd_wand_l E1 E2 P Q : (P -∗ Q) ∗ (MUpd E1 E2 P) ⊢ MUpd E1 E2 Q.
+  Proof. rewrite MUpd_frame_l. rewrite wand_elim_l. auto. Qed.
+  Lemma MUpd_wand_r E1 E2 P Q : (MUpd E1 E2 P) ∗ (P -∗ Q) ⊢ MUpd E1 E2 Q.
+  Proof. rewrite MUpd_frame_r. rewrite wand_elim_r. auto. Qed.
+
+  Lemma MUpd_trans_frame E1 E2 E3 P Q :
+    ((Q -* MUpd E2 E3 emp) ∗ MUpd E1 E2 (Q ∗ P)) ⊢ MUpd E1 E3 P.
+  Proof.
+    rewrite MUpd_frame_l.
+    rewrite MUpd_frame_r.
+
+assoc -(comm _ Q) wand_elim_r.
+    by rewrite fupd_frame_r left_id fupd_trans.
+  Qed.
+
+  Lemma fupd_elim E1 E2 E3 P Q :
+    (Q -∗ (|={E2,E3}=> P)) → (|={E1,E2}=> Q) -∗ (|={E1,E3}=> P).
+  Proof. intros ->. rewrite fupd_trans //. Qed.
+
+  Lemma fupd_mask_frame_r E1 E2 Ef P :
+    E1 ## Ef → (|={E1,E2}=> P) ={E1 ∪ Ef,E2 ∪ Ef}=∗ P.
+  Proof.
+    intros ?. rewrite -fupd_mask_frame_r' //. f_equiv.
+    apply impl_intro_l, and_elim_r.
+  Qed.
+  Lemma fupd_mask_mono E1 E2 P : E1 ⊆ E2 → (|={E1}=> P) ={E2}=∗ P.
+  Proof.
+    intros (Ef&->&?)%subseteq_disjoint_union_L. by apply fupd_mask_frame_r.
+  Qed.
+  (** How to apply an arbitrary mask-changing view shift when having
+      an arbitrary mask. *)
+  Lemma fupd_mask_frame E E' E1 E2 P :
+    E1 ⊆ E →
+    (|={E1,E2}=> |={E2 ∪ (E ∖ E1),E'}=> P) -∗ (|={E,E'}=> P).
+  Proof.
+    intros ?. rewrite (fupd_mask_frame_r _ _ (E ∖ E1)); last set_solver.
+    rewrite fupd_trans.
+    by replace (E1 ∪ E ∖ E1) with E by (by apply union_difference_L).
+  Qed.
+  (* A variant of [fupd_mask_frame] that works well for accessors: Tailored to
+     eliminate updates of the form [|={E1,E1∖E2}=> Q] and provides a way to
+     transform the closing view shift instead of letting you prove the same
+     side-conditions twice. *)
+  Lemma fupd_mask_frame_acc E E' E1(*Eo*) E2(*Em*) P Q :
+    E1 ⊆ E →
+    (|={E1,E1∖E2}=> Q) -∗
+    (Q -∗ |={E∖E2,E'}=> (∀ R, (|={E1∖E2,E1}=> R) -∗ |={E∖E2,E}=> R) -∗  P) -∗
+    (|={E,E'}=> P).
+  Proof.
+    intros HE. apply wand_intro_r. rewrite fupd_frame_r.
+    rewrite wand_elim_r. clear Q.
+    rewrite -(fupd_mask_frame E E'); first apply fupd_mono; last done.
+    (* The most horrible way to apply fupd_intro_mask *)
+    rewrite -[X in (X -∗ _)](right_id emp%I).
+    rewrite (fupd_mask_intro_subseteq (E1 ∖ E2 ∪ E ∖ E1) (E ∖ E2) emp); last first.
+    { rewrite {1}(union_difference_L _ _ HE). set_solver. }
+    rewrite fupd_frame_l fupd_frame_r. apply fupd_elim.
+    apply fupd_mono.
+    eapply wand_apply;
+      last (apply sep_mono; first reflexivity); first reflexivity.
+    apply forall_intro=>R. apply wand_intro_r.
+    rewrite fupd_frame_r. apply fupd_elim. rewrite left_id.
+    rewrite (fupd_mask_frame_r _ _ (E ∖ E1)); last set_solver+.
+    rewrite {4}(union_difference_L _ _ HE). done.
+  Qed.
+
+  Lemma fupd_mask_subseteq_emptyset_difference E1 E2 :
+    E2 ⊆ E1 →
+    ⊢@{PROP} |={E1, E2}=> |={∅, E1∖E2}=> emp.
+  Proof.
+    intros ?. rewrite [in fupd E1](union_difference_L E2 E1); [|done].
+    rewrite (comm_L (∪))
+      -[X in fupd _ X](left_id_L ∅ (∪) E2) -fupd_mask_frame_r; [|set_solver+].
+    apply fupd_mask_intro_subseteq; set_solver.
+  Qed.
+
+  Lemma fupd_or E1 E2 P Q :
+    (|={E1,E2}=> P) ∨ (|={E1,E2}=> Q) ⊢@{PROP}
+    (|={E1,E2}=> (P ∨ Q)).
+  Proof. apply or_elim; apply fupd_mono; [ apply or_intro_l | apply or_intro_r ]. Qed.
+
+  Global Instance fupd_or_homomorphism E :
+    MonoidHomomorphism bi_or bi_or (flip (⊢)) (fupd (PROP:=PROP) E E).
+  Proof. split; [split|]; try apply _; [apply fupd_or | apply fupd_intro]. Qed.
+
+  Lemma fupd_and E1 E2 P Q :
+    (|={E1,E2}=> (P ∧ Q)) ⊢@{PROP} (|={E1,E2}=> P) ∧ (|={E1,E2}=> Q).
+  Proof. apply and_intro; apply fupd_mono; [apply and_elim_l | apply and_elim_r]. Qed.
+
+  Lemma fupd_exist E1 E2 A (Φ : A → PROP) : (∃ x : A, |={E1, E2}=> Φ x) ⊢ |={E1, E2}=> ∃ x : A, Φ x.
+  Proof. apply exist_elim=> a. by rewrite -(exist_intro a). Qed.
+
+  Lemma fupd_forall E1 E2 A (Φ : A → PROP) : (|={E1, E2}=> ∀ x : A, Φ x) ⊢ ∀ x : A, |={E1, E2}=> Φ x.
+  Proof. apply forall_intro=> a. by rewrite -(forall_elim a). Qed.
+
+  Lemma fupd_sep E P Q : (|={E}=> P) ∗ (|={E}=> Q) ={E}=∗ P ∗ Q.
+  Proof. by rewrite fupd_frame_r fupd_frame_l fupd_trans. Qed.
+
+  Global Instance fupd_sep_homomorphism E :
+    MonoidHomomorphism bi_sep bi_sep (flip (⊢)) (fupd (PROP:=PROP) E E).
+  Proof. split; [split|]; try apply _; [apply fupd_sep | apply fupd_intro]. Qed.
+
+
+
+
+
+
+
+
 Module Region.
   Section REGION.
     Variable A: Type.
@@ -775,87 +1227,6 @@ Module Region.
     Qed.
 
     Variable interp: A -> iProp.
-
-    Definition sat_list (l: list A): iProp :=
-      fold_right (fun a P => interp a ** P) True%I l.
-
-    Lemma sat_list_nil
-      :
-      ⊢ sat_list [].
-    Proof.
-      unfold sat_list. ss. auto.
-    Qed.
-
-    Lemma sat_list_cons_fold hd tl
-      :
-      (interp hd ** sat_list tl)
-        -∗
-        (sat_list (hd::tl)).
-    Proof.
-      unfold sat_list. ss.
-    Qed.
-
-    Lemma sat_list_cons_unfold hd tl
-      :
-      (sat_list (hd::tl))
-        -∗
-        (interp hd ** sat_list tl).
-    Proof.
-      unfold sat_list. ss.
-    Qed.
-
-    Lemma sat_list_split l0 l1
-      :
-      (sat_list (l0 ++ l1))
-        -∗
-        (sat_list l0 ** sat_list l1).
-    Proof.
-      induction l0; ss.
-      { iIntros "SAT". iFrame. }
-      { iIntros "[INTERP SAT]". iFrame. iApply IHl0; auto. }
-    Qed.
-
-    Lemma sat_list_combine l0 l1
-      :
-      (sat_list l0 ** sat_list l1)
-        -∗
-        (sat_list (l0 ++ l1)).
-    Proof.
-      induction l0; ss.
-      { iIntros "[_ SAT]". auto. }
-      { iIntros "[[INTERP SAT0] SAT1]". iFrame.
-        iApply IHl0. iFrame.
-      }
-    Qed.
-
-    Lemma sat_list_add l a
-      :
-      (interp a ** sat_list l)
-        -∗
-        (sat_list (l++[a])).
-    Proof.
-      iIntros "[NEW SAT]". iApply sat_list_combine. iFrame.
-    Qed.
-
-    Lemma sat_list_update l k a
-          (FIND: nth_error l k = Some a)
-      :
-      sat_list l ⊢ interp a ** (interp a -* sat_list l).
-    Proof.
-      hexploit nth_error_split; eauto. i. des. subst.
-      iIntros "SAT". iPoseProof (sat_list_split with "SAT") as "[SAT0 SAT1]".
-      iPoseProof (sat_list_cons_unfold with "SAT1") as "[OLD SAT1]".
-      iFrame. iIntros "NEW". iApply sat_list_combine. iFrame.
-    Qed.
-
-    Lemma sat_list_nth_sub l k a
-          (FIND: nth_error l k = Some a)
-      :
-      ⊢ SubIProp (interp a) (sat_list l).
-    Proof.
-      iIntros "H". iPoseProof (sat_list_update with "H") as "[H0 H1]"; eauto.
-      iFrame. iModIntro. iIntros "H". iModIntro. iApply ("H1" with "H").
-    Qed.
 
     Definition sat: iProp := ∃ l, black l ** sat_list l.
 
@@ -936,3 +1307,198 @@ Module Region.
     Qed.
   End REGION.
 End Region.
+
+
+
+
+Section class_instances_updates.
+Context {PROP : bi}.
+Implicit Types P Q R : PROP.
+
+Global Instance from_assumption_bupd `{!BiBUpd PROP} p P Q :
+  FromAssumption p P Q → KnownRFromAssumption p P (|==> Q).
+Proof. rewrite /KnownRFromAssumption /FromAssumption=>->. apply bupd_intro. Qed.
+Global Instance from_assumption_fupd
+    `{!BiBUpd PROP, !BiFUpd PROP, !BiBUpdFUpd PROP} E p P Q :
+  FromAssumption p P (|==> Q) → KnownRFromAssumption p P (|={E}=> Q).
+Proof. rewrite /KnownRFromAssumption /FromAssumption=>->. apply bupd_fupd. Qed.
+
+Global Instance from_pure_bupd `{!BiBUpd PROP} a P φ :
+  FromPure a P φ → FromPure a (|==> P) φ.
+Proof. rewrite /FromPure=> <-. apply bupd_intro. Qed.
+Global Instance from_pure_fupd `{!BiFUpd PROP} a E P φ :
+  FromPure a P φ → FromPure a (|={E}=> P) φ.
+Proof. rewrite /FromPure=> <-. apply fupd_intro. Qed.
+
+Global Instance into_wand_bupd `{!BiBUpd PROP} p q R P Q :
+  IntoWand false false R P Q → IntoWand p q (|==> R) (|==> P) (|==> Q).
+Proof.
+  rewrite /IntoWand /= => HR. rewrite !intuitionistically_if_elim HR.
+  apply wand_intro_l. by rewrite bupd_sep wand_elim_r.
+Qed.
+Global Instance into_wand_fupd `{!BiFUpd PROP} E p q R P Q :
+  IntoWand false false R P Q →
+  IntoWand p q (|={E}=> R) (|={E}=> P) (|={E}=> Q).
+Proof.
+  rewrite /IntoWand /= => HR. rewrite !intuitionistically_if_elim HR.
+  apply wand_intro_l. by rewrite fupd_sep wand_elim_r.
+Qed.
+
+Global Instance into_wand_bupd_persistent `{!BiBUpd PROP} p q R P Q :
+  IntoWand false q R P Q → IntoWand p q (|==> R) P (|==> Q).
+Proof.
+  rewrite /IntoWand /= => HR. rewrite intuitionistically_if_elim HR.
+  apply wand_intro_l. by rewrite bupd_frame_l wand_elim_r.
+Qed.
+Global Instance into_wand_fupd_persistent `{!BiFUpd PROP} E1 E2 p q R P Q :
+  IntoWand false q R P Q → IntoWand p q (|={E1,E2}=> R) P (|={E1,E2}=> Q).
+Proof.
+  rewrite /IntoWand /= => HR. rewrite intuitionistically_if_elim HR.
+  apply wand_intro_l. by rewrite fupd_frame_l wand_elim_r.
+Qed.
+
+Global Instance into_wand_bupd_args `{!BiBUpd PROP} p q R P Q :
+  IntoWand p false R P Q → IntoWand' p q R (|==> P) (|==> Q).
+Proof.
+  rewrite /IntoWand' /IntoWand /= => ->.
+  apply wand_intro_l. by rewrite intuitionistically_if_elim bupd_wand_r.
+Qed.
+Global Instance into_wand_fupd_args `{!BiFUpd PROP} E1 E2 p q R P Q :
+  IntoWand p false R P Q → IntoWand' p q R (|={E1,E2}=> P) (|={E1,E2}=> Q).
+Proof.
+  rewrite /IntoWand' /IntoWand /= => ->.
+  apply wand_intro_l. by rewrite intuitionistically_if_elim fupd_wand_r.
+Qed.
+
+Global Instance from_sep_bupd `{!BiBUpd PROP} P Q1 Q2 :
+  FromSep P Q1 Q2 → FromSep (|==> P) (|==> Q1) (|==> Q2).
+Proof. rewrite /FromSep=><-. apply bupd_sep. Qed.
+Global Instance from_sep_fupd `{!BiFUpd PROP} E P Q1 Q2 :
+  FromSep P Q1 Q2 → FromSep (|={E}=> P) (|={E}=> Q1) (|={E}=> Q2).
+Proof. rewrite /FromSep =><-. apply fupd_sep. Qed.
+
+Global Instance from_or_bupd `{!BiBUpd PROP} P Q1 Q2 :
+  FromOr P Q1 Q2 → FromOr (|==> P) (|==> Q1) (|==> Q2).
+Proof. rewrite /FromOr=><-. apply bupd_or. Qed.
+Global Instance from_or_fupd `{!BiFUpd PROP} E1 E2 P Q1 Q2 :
+  FromOr P Q1 Q2 → FromOr (|={E1,E2}=> P) (|={E1,E2}=> Q1) (|={E1,E2}=> Q2).
+Proof. rewrite /FromOr=><-. apply fupd_or. Qed.
+
+Global Instance into_and_bupd `{!BiBUpd PROP} P Q1 Q2 :
+  IntoAnd false P Q1 Q2 → IntoAnd false (|==> P) (|==> Q1) (|==> Q2).
+Proof. rewrite /IntoAnd/==>->. apply bupd_and. Qed.
+Global Instance into_and_fupd `{!BiFUpd PROP} E1 E2 P Q1 Q2 :
+  IntoAnd false P Q1 Q2 → IntoAnd false (|={E1,E2}=> P) (|={E1,E2}=> Q1) (|={E1,E2}=> Q2).
+Proof. rewrite /IntoAnd/==>->. apply fupd_and. Qed.
+
+Global Instance from_exist_bupd `{!BiBUpd PROP} {A} P (Φ : A → PROP) :
+  FromExist P Φ → FromExist (|==> P) (λ a, |==> Φ a)%I.
+Proof. rewrite /FromExist=><-. apply bupd_exist. Qed.
+Global Instance from_exist_fupd `{!BiFUpd PROP} {A} E1 E2 P (Φ : A → PROP) :
+  FromExist P Φ → FromExist (|={E1,E2}=> P) (λ a, |={E1,E2}=> Φ a)%I.
+Proof. rewrite /FromExist=><-. apply fupd_exist. Qed.
+
+Global Instance into_forall_bupd `{!BiBUpd PROP} {A} P (Φ : A → PROP) :
+  IntoForall P Φ → IntoForall (|==> P) (λ a, |==> Φ a)%I.
+Proof. rewrite /IntoForall=>->. apply bupd_forall. Qed.
+Global Instance into_forall_fupd `{!BiFUpd PROP} {A} E1 E2 P (Φ : A → PROP) :
+  IntoForall P Φ → IntoForall (|={E1,E2}=> P) (λ a, |={E1,E2}=> Φ a)%I.
+Proof. rewrite /IntoForall=>->. apply fupd_forall. Qed.
+
+Global Instance from_forall_fupd
+    `{!BiFUpd PROP, !BiPlainly PROP, !BiFUpdPlainly PROP} E1 E2 {A} P (Φ : A → PROP) name :
+  (* Some cases in which [E2 ⊆ E1] holds *)
+  TCOr (TCEq E1 E2) (TCOr (TCEq E1 ⊤) (TCEq E2 ∅)) →
+  FromForall P Φ name → (∀ x, Plain (Φ x)) →
+  FromForall (|={E1,E2}=> P) (λ a, |={E1,E2}=> (Φ a))%I name.
+Proof.
+  rewrite /FromForall=> -[->|[->|->]] <- ?; rewrite fupd_plain_forall; set_solver.
+Qed.
+Global Instance from_forall_step_fupd
+    `{!BiFUpd PROP, !BiPlainly PROP, !BiFUpdPlainly PROP} E1 E2 {A} P (Φ : A → PROP) name :
+  (* Some cases in which [E2 ⊆ E1] holds *)
+  TCOr (TCEq E1 E2) (TCOr (TCEq E1 ⊤) (TCEq E2 ∅)) →
+  FromForall P Φ name → (∀ x, Plain (Φ x)) →
+  FromForall (|={E1}[E2]▷=> P) (λ a, |={E1}[E2]▷=> (Φ a))%I name.
+Proof.
+  rewrite /FromForall=> -[->|[->|->]] <- ?; rewrite step_fupd_plain_forall; set_solver.
+Qed.
+
+Global Instance is_except_0_bupd `{!BiBUpd PROP} P : IsExcept0 P → IsExcept0 (|==> P).
+Proof.
+  rewrite /IsExcept0=> HP.
+  by rewrite -{2}HP -(except_0_idemp P) -except_0_bupd -(except_0_intro P).
+Qed.
+Global Instance is_except_0_fupd `{!BiFUpd PROP} E1 E2 P :
+  IsExcept0 (|={E1,E2}=> P).
+Proof. by rewrite /IsExcept0 except_0_fupd. Qed.
+
+Global Instance from_modal_bupd `{!BiBUpd PROP} P :
+  FromModal True modality_id (|==> P) (|==> P) P.
+Proof. by rewrite /FromModal /= -bupd_intro. Qed.
+Global Instance from_modal_fupd E P `{!BiFUpd PROP} :
+  FromModal True modality_id (|={E}=> P) (|={E}=> P) P.
+Proof. by rewrite /FromModal /= -fupd_intro. Qed.
+Global Instance from_modal_fupd_wrong_mask E1 E2 P `{!BiFUpd PROP} :
+  FromModal
+        (pm_error "Only non-mask-changing update modalities can be introduced directly.
+Use [iApply fupd_mask_intro] to introduce mask-changing update modalities")
+    modality_id (|={E1,E2}=> P) (|={E1,E2}=> P) P | 100.
+Proof. by intros []. Qed.
+
+Global Instance elim_modal_bupd `{!BiBUpd PROP} p P Q :
+  ElimModal True p false (|==> P) P (|==> Q) (|==> Q).
+Proof.
+  by rewrite /ElimModal
+    intuitionistically_if_elim bupd_frame_r wand_elim_r bupd_trans.
+Qed.
+
+Global Instance elim_modal_bupd_plain_goal
+    `{!BiBUpd PROP, !BiPlainly PROP, !BiBUpdPlainly PROP} p P Q :
+  Plain Q → ElimModal True p false (|==> P) P Q Q.
+Proof.
+  intros. by rewrite /ElimModal intuitionistically_if_elim
+    bupd_frame_r wand_elim_r bupd_plain.
+Qed.
+Global Instance elim_modal_bupd_plain
+    `{!BiBUpd PROP, !BiPlainly PROP, !BiBUpdPlainly PROP} p P Q :
+  Plain P → ElimModal True p p (|==> P) P Q Q.
+Proof. intros. by rewrite /ElimModal bupd_plain wand_elim_r. Qed.
+Global Instance elim_modal_bupd_fupd
+    `{!BiBUpd PROP, !BiFUpd PROP, !BiBUpdFUpd PROP} p E1 E2 P Q :
+  ElimModal True p false (|==> P) P (|={E1,E2}=> Q) (|={E1,E2}=> Q) | 10.
+Proof.
+  by rewrite /ElimModal intuitionistically_if_elim
+    (bupd_fupd E1) fupd_frame_r wand_elim_r fupd_trans.
+Qed.
+Global Instance elim_modal_fupd_fupd `{!BiFUpd PROP} p E1 E2 E3 P Q :
+  ElimModal True p false (|={E1,E2}=> P) P (|={E1,E3}=> Q) (|={E2,E3}=> Q).
+Proof.
+  by rewrite /ElimModal intuitionistically_if_elim
+    fupd_frame_r wand_elim_r fupd_trans.
+Qed.
+Global Instance elim_modal_fupd_fupd_wrong_mask `{!BiFUpd PROP} p E0 E1 E2 E3 P Q :
+  ElimModal
+    (pm_error "Goal and eliminated modality must have the same mask.
+Use [iMod (fupd_mask_subseteq E2)] to adjust the mask of your goal to [E2]")
+    p false
+    (|={E1,E2}=> P) False (|={E0,E3}=> Q) False | 100.
+Proof. intros []. Qed.
+
+Global Instance add_modal_bupd `{!BiBUpd PROP} P Q : AddModal (|==> P) P (|==> Q).
+Proof. by rewrite /AddModal bupd_frame_r wand_elim_r bupd_trans. Qed.
+
+Global Instance add_modal_fupd `{!BiFUpd PROP} E1 E2 P Q :
+  AddModal (|={E1}=> P) P (|={E1,E2}=> Q).
+Proof. by rewrite /AddModal fupd_frame_r wand_elim_r fupd_trans. Qed.
+
+Global Instance elim_acc_fupd `{!BiFUpd PROP} {X} E1 E2 E α β mγ Q :
+  ElimAcc (X:=X) True (fupd E1 E2) (fupd E2 E1) α β mγ
+          (|={E1,E}=> Q)
+          (λ x, |={E2}=> β x ∗ (mγ x -∗? |={E1,E}=> Q))%I.
+Proof.
+  iIntros (_) "Hinner >Hacc". iDestruct "Hacc" as (x) "[Hα Hclose]".
+  iMod ("Hinner" with "Hα") as "[Hβ Hfin]".
+  iMod ("Hclose" with "Hβ") as "Hγ". by iApply "Hfin".
+Qed.
+End class_instances_updates.
